Simplify the system to an injective PTS

syntax.sig
@@ -3,7 +3,7 @@ nat : Type
 
 Univ : nat -> tm
 Lam : tm -> (tm -> tm) -> tm
-App : tm -> (tm -> tm) -> tm -> tm -> tm
+App : (tm -> tm) -> tm -> tm -> tm
 Pi : tm -> (tm -> tm) -> tm
 TmUnit : tm
 TyUnit : tm
